theory/CoreRel/Hoare.v
@@ -1,0 +1,226 @@
+From Common Require Import Id Fixpoints.
+From Coq Require Import Bool.Bool.
+From Coq Require Import Arith.Arith.
+From Coq Require Import Arith.EqNat.
+From Coq Require Import Arith.PeanoNat. Import Nat.
+From Coq Require Import Lia.
+From Coq Require Import Strings.String.
+From Imp Require Import Syntax Semantics Equiv.
+
+Import ListNotations.
+
+From Common Require Import Id Fixpoints.
+
+From stdpp Require Export prelude fin_maps fin_map_dom.
+From Imp Require Import Syntax.
+
+Import Imp.Syntax.notations.
+Import Imp.Semantics.notations.
+
+Section Definitions.
+(* The type of variable identifiers. *)
+Definition I := @prod_I string.
+Context {M : Type -> Type}.
+Context {id : Id I (@prod_M M)}.
+
+Definition state := (@prod_M M) nat.
+
+Definition Assertion := state -> Prop.
+
+Definition assert_implies (P Q : Assertion) : Prop :=
+  forall st, P st -> Q st.
+
+Declare Scope hoare_spec_scope.
+Notation "P ->> Q" := (assert_implies P Q) (at level 80) : hoare_spec_scope.
+Open Scope hoare_spec_scope.
+Notation "P <<->> Q" :=
+  (P ->> Q /\ Q ->> P) (at level 80) : hoare_spec_scope. 
+
+
+Definition Aexp : Type := state -> nat.
+
+Definition assert_of_Prop (P : Prop) : Assertion := fun _ => P.
+Definition Aexp_of_nat (n : nat) : Aexp := fun _ => n.
+
+Definition Aexp_of_aexp (a : aexp) : Aexp := fun st => aeval st a.
+
+Coercion assert_of_Prop : Sortclass >-> Assertion.
+Coercion Aexp_of_nat : nat >-> Aexp.
+Coercion Aexp_of_aexp : aexp >-> Aexp.
+Add Printing Coercion Aexp_of_nat Aexp_of_aexp assert_of_Prop.
+
+Arguments assert_of_Prop /.
+Arguments Aexp_of_nat /.
+Arguments Aexp_of_aexp /.
+Add Printing Coercion Aexp_of_nat Aexp_of_aexp assert_of_Prop.
+
+Declare Scope assertion_scope.
+Bind Scope assertion_scope with Assertion.
+Bind Scope assertion_scope with Aexp.
+Delimit Scope assertion_scope with assertion.
+
+Notation assert P := (P%assertion : Assertion).
+Notation mkAexp a := (a%assertion : Aexp).
+
+Notation "~ P" := (fun st => ~ assert P st) : assertion_scope.
+Notation "P /\ Q" := (fun st => assert P st /\ assert Q st) : assertion_scope.
+Notation "P \/ Q" := (fun st => assert P st \/ assert Q st) : assertion_scope.
+Notation "P -> Q" := (fun st => assert P st ->  assert Q st) : assertion_scope.
+Notation "P <-> Q" := (fun st => assert P st <->  assert Q st) : assertion_scope.
+Notation "a = b" := (fun st => mkAexp a st = mkAexp b st) : assertion_scope.
+Notation "a <> b" := (fun st => mkAexp a st <> mkAexp b st) : assertion_scope.
+Notation "a <= b" := (fun st => mkAexp a st <= mkAexp b st) : assertion_scope.
+Notation "a < b" := (fun st => mkAexp a st < mkAexp b st) : assertion_scope.
+Notation "a >= b" := (fun st => mkAexp a st >= mkAexp b st) : assertion_scope.
+Notation "a > b" := (fun st => mkAexp a st > mkAexp b st) : assertion_scope.
+Notation "a + b" := (fun st => mkAexp a st + mkAexp b st) : assertion_scope.
+Notation "a - b" := (fun st => mkAexp a st - mkAexp b st) : assertion_scope.
+Notation "a * b" := (fun st => mkAexp a st * mkAexp b st) : assertion_scope.
+
+
+Definition ap {X} (f : nat -> X) (x : Aexp) :=
+  fun st => f (x st).
+
+Definition ap2 {X} (f : nat -> nat -> X) (x : Aexp) (y : Aexp) (st : state) :=
+  f (x st) (y st).
+
+
+Definition hoare_triple
+           (P : Assertion) (c : @com I) (Q : Assertion) : Prop :=
+  forall st st',
+     P st  ->
+      st =[ c ]=> st' ->
+     Q st'.
+
+Notation "{{ P }}  c  {{ Q }}" :=
+  (hoare_triple P c Q) (at level 90, c custom com at level 99)
+  : hoare_spec_scope.
+
+
+Definition assn_sub X a (P:Assertion) : Assertion :=
+  fun (st : state) => 
+    P (<[X := aeval st a]> st).
+
+Set Printing All.
+Print assn_sub.
+Unset Printing All.
+
+Notation "P [ X |-> a ]" := (assn_sub X a P)
+  (at level 10, X at next level, a custom com) : hoare_spec_scope.
+
+
+(*skip rule*)
+Theorem hoare_skip : forall P,
+     hoare_triple P <{skip}> P.
+Proof.
+  unfold hoare_triple. intros. inversion H0; subst. assumption.
+Qed.
+
+(*sequence*)
+Theorem hoare_seq : forall P Q R r1 r2,
+     hoare_triple Q r2 R ->
+     hoare_triple P r1 Q ->
+     hoare_triple P <{r1; r2}> R.
+Proof.
+ unfold hoare_triple; intros. inversion H2; subst. eapply H0 in H1.
+ eapply H. eassumption. eassumption. eassumption.
+Qed.
+
+(*hoare_triple (assn_sub X a Q) X := a Q*)
+Theorem hoare_asgn : forall Q X a, 
+  hoare_triple (assn_sub X a Q) <{X := a}> Q.
+Proof.
+unfold hoare_triple, assn_sub. intros. inversion H0; subst. 
+assumption.
+Qed.
+
+Hint Unfold assert_implies hoare_triple assn_sub insert : core.
+Hint Unfold assert_of_Prop Aexp_of_nat Aexp_of_aexp : core.
+
+(*assn_auto, assn_auto''*)
+Ltac assn_auto :=
+  try auto; 
+  try (unfold "->>", assn_sub, insert;
+       intros; simpl in *; lia).
+
+Print assn_auto.
+
+
+
+(*strengthen precc.*)
+Theorem hoare_consequence_pre : forall (P P' Q : Assertion) r,
+  hoare_triple P' r Q ->
+  assert_implies P P' ->
+  hoare_triple P r Q. 
+Proof.
+ unfold hoare_triple, "->>".
+  intros P P' Q c Hhoare Himp st st' Heval Hpre.
+  eapply Hhoare. eapply Himp. eassumption. assumption.
+Qed.
+
+(*weaken post.*)
+Theorem hoare_consequence_post : forall (P Q Q' : Assertion) r,
+  hoare_triple P r Q' ->
+  assert_implies Q' Q ->
+  hoare_triple P r Q. 
+Proof.
+ unfold hoare_triple, "->>". intros.
+ eapply H0. eapply H. eassumption. assumption.
+Qed.
+
+
+Definition bassn b : Assertion :=
+  fun st => (beval st b = true).
+
+Coercion bassn : bexp >-> Assertion.
+
+Arguments bassn /.
+
+Ltac assn_auto' :=
+  unfold "->>", assn_sub, insert, bassn;
+  intros; simpl in *;
+  try rewrite -> eqb_eq in *; (* for equalities *)
+  auto; try lia.
+
+Ltac assn_auto'' :=
+  unfold "->>", assn_sub, insert, bassn;
+  intros; simpl in *;
+  try rewrite -> eqb_eq in *;
+  try rewrite -> leb_le in *;  (* for inequalities *)
+  auto; try lia.
+
+(** A useful fact about [bassn]: *)
+
+Lemma bexp_eval_false : forall b st,
+  beval st b = false -> ~ ((bassn b) st).
+Proof. congruence. Qed.
+
+Hint Resolve bexp_eval_false : core.
+
+(*hoare_if*)
+Theorem hoare_if : forall P Q (b:bexp) r1 r2,
+  hoare_triple (P /\ b) r1 Q ->
+  hoare_triple (P /\ ~ b) r2 Q ->
+  hoare_triple P <{if b then r1 else r2 end}> Q.
+Proof.
+unfold hoare_triple; intros.
+inversion H2; subst. eapply H. eauto.
+assumption. eauto.
+Qed.
+
+(*hoare_while*)
+Theorem hoare_while : forall P (b: bexp) r,
+  hoare_triple (P /\ b) r P ->
+  hoare_triple P <{while b do r end}> (P /\ ~ b).
+Proof.
+unfold hoare_triple; intros. 
+remember <{while b do r end}> as original_command eqn:Horig.
+induction H1. discriminate. discriminate. discriminate. discriminate.
+discriminate. inversion Horig; subst. eauto. 
+inversion Horig; subst. eauto.
+Qed.
+
+End Definitions.
+
+
+
